thys/LLL_Basis_Reduction/FPLLL_Solver.thy
@@ -1,0 +1,147 @@
+(*
+    Authors:    Sebastiaan Joosten
+                René Thiemann
+*)
+subsection \<open>A Haskell Interface to the FPLLL-Solver\<close>
+
+theory FPLLL_Solver
+  imports LLL_Certification
+begin
+
+text \<open>We define @{const external_lll_solver} via an invocation of the fplll solver.
+  For eta we use the default value of fplll, and delta is chosen so that 
+  the required precision of alpha will be guaranteed. We use the command-line
+  option -bvu in order to get the witnesses that are required for certification.\<close>
+
+text \<open>Warning: Since we only define a Haskell binding for FPLLL, 
+  the target languages do no longer evaluate to the same results on @{const short_vector_hybrid}!\<close>
+
+code_printing
+  code_module "FPLLL_Solver" \<rightharpoonup> (Haskell) \<open>
+import System.IO.Unsafe (unsafePerformIO);
+import System.IO (stderr,hPutStrLn,hPutStr);
+import System.Process (readProcessWithExitCode);
+import GHC.IO.Exception (ExitCode(ExitSuccess));
+import Data.Char (isNumber, isSpace);
+import Data.List (intercalate);
+
+fplll_command :: String;
+fplll_command = "fplll";
+
+default_eta :: Double;
+default_eta = 0.51;
+
+alpha_to_delta :: (Integer,Integer) -> Double;
+alpha_to_delta (num,denom) = (fromIntegral denom / fromIntegral num) + 
+  (default_eta * default_eta);
+
+showrow :: [Integer] -> String;
+showrow rowA = "["++ intercalate " " (map show rowA) ++ "]";
+showmat :: [[Integer]] -> String;
+showmat matA = "["++ intercalate "\n " (map showrow matA) ++"]";
+
+
+fplll_solver :: (Integer,Integer) -> [[Integer]] -> ([[Integer]],([[Integer]],[[Integer]]));
+fplll_solver alpha in_mat = unsafePerformIO $ do {
+  (code,res,err) <- readProcessWithExitCode fplll_command ["-e", show default_eta, "-d", show (alpha_to_delta alpha), "-of", "bvu"] (showmat in_mat);
+  if code == ExitSuccess && err == ""
+    then parseRes res
+    else hPutStr stderr err >> fail_to_execute }
+ where {
+   parseMat ('[':as) = do {
+     rem0 <- parseSpaces as;
+     (rows,rem1) <- parseRows rem0;
+     case rem1 of
+       ']':rem2 -> do {
+         rem3 <- parseSpaces rem2;
+         return (rows,rem3)
+         };
+       _ -> abort$ "Expecting closing ']' while parsing a matrix.\n"
+       };
+   parseMat _ = abort "Expecting opening '[' while parsing a matrix";
+   parseRows ('[':rem0) = do {
+     rem1 <- parseSpaces rem0;
+     (nums,rem2)<-parseNums rem1;
+     case rem2 of
+       ']':rem3 -> do { rem4 <- parseSpaces rem3;
+                        (rows,rem5) <- parseRows rem4;
+                        return (map read nums:rows,rem5) }
+       _ -> abort$ "Expecting closing ']' while parsing a row\n" ++ rem2
+       };
+   parseRows x = return ([],x);
+   parseNums o@(a:rem0) =
+     if isNumber a || a == '-' then do {
+       (num,rem1) <- parseNum rem0;
+       rem2 <- parseSpaces rem1;
+       (nums,rem3) <- parseNums rem2;
+       return ((a:num):nums,rem3) }
+     else if isSpace a then do {
+       rem1 <- parseSpaces rem0;
+       parseNums rem1}
+     else return ([],o);
+   parseNums [] = return ([],[]);
+   parseNum o@(a:rem0) =
+     if isNumber a then do {
+       (num,rem1) <- parseNum rem0;
+       return (a:num,rem1) 
+       }
+     else return ([],o);
+   parseNum o = return ([],o);
+   parseSpaces o@(a:as) = if isSpace a then parseSpaces as else return o;
+   parseSpaces [] = return [];
+   parseRes :: String -> IO ([[Integer]], ([[Integer]], [[Integer]]));
+   parseRes res = do {
+     rem0 <- parseSpaces res;
+     if length rem0 <= 0
+       then default_answer
+       else do {
+         (m1,rem1) <- parseMat rem0;
+         (m2,rem2) <- parseMat rem1;
+         (m3,rem3) <- parseMat rem2;
+          if length rem3 > 0
+            then abort "Unexpected output after parsing three matrices."
+            else return (m1,(m2,m3))
+            }
+        };
+   fail_to_execute = seq sendError default_answer;
+   
+   default_answer = -- not small enough, but it'll be accepted
+     return (in_mat,(id_ofsize (length in_mat),id_ofsize (length in_mat)));
+   abort str = error$ "Runtime exception in parsing fplll output:\n"++str;
+   };
+   
+
+sendError :: (); -- bad trick using unsafeIO to make this error only appear once. I believe this is OK since the error is non-critical and the 'only appear once' is non-critical too.
+sendError = unsafePerformIO $ do {
+  hPutStrLn stderr "--- WARNING ---";
+  hPutStrLn stderr "Failed to run fplll.";
+  hPutStrLn stderr "To remove this warning, either:";
+  hPutStrLn stderr "  - install fplll and ensure it is in your path.";
+  hPutStrLn stderr "  - create an executable fplll that always returns successfully without generating output.";
+  hPutStrLn stderr "Installing fplll correctly helps to reduce time spent verifying your certificate.";
+  hPutStrLn stderr "--- END OF WARNING ---"
+  };
+
+id_ofsize :: Int -> [[Integer]];
+id_ofsize n = [[if i == j then 1 else 0 | j <- [0..n-1]] | i <- [0..n-1]];
+\<close>
+
+code_reserved Haskell FPLLL_Solver fplll_solver
+
+code_printing
+  constant external_lll_solver \<rightharpoonup> (Haskell) "FPLLL'_Solver.fplll'_solver"
+| constant enable_external_lll_solver \<rightharpoonup> (Haskell) "True"
+
+text \<open>Note that since we only enabled the external LLL solver for Haskell, the result of 
+  @{const short_vector_hybrid} will usually differ when executed in Haskell in
+  comparison to any of the other target languages. For instance, consider the 
+  invocation of:\<close>
+
+value (code) "short_vector_test_hybrid [[1,4903,4902], [0,39023,0], [0,0,39023]]" 
+
+text \<open>The above value-command evaluates the expression in Eval/SML to 77714 (by computing
+  a short vector solely by the verified @{const short_vector} algorithm, whereas
+  the generated Haskell-code via the external LLL solver yields 60414!\<close>
+
+(* export_code short_vector_test_hybrid in Haskell module_name LLL file "~/Code" *)
+end
